theories/lang/cpp/syntax/names.v
@@ -43,14 +43,21 @@ Definition localname : Set := ident.
 Bind Scope bs_scope with localname.
 #[global] Instance localname_eq: EqDecision localname := _.
 
-(**
-Identify an aggregate field.
-XXX: is this used for function members? If so, rename.
-[Member] is taken, but [member_name] or shortenings of
-[member_qualified_name] could work. *)
+(** Identify an aggregate field.
+
+   TODO (JH): this will need to be generalized to support pointer-to-member functions;
+     rename when we subsequently generalize member pointer support.
+
+     [Member] is taken, but [member_name] or shortenings of
+     [member_qualified_name] could work.
+ *)
 Record field : Set :=
 { f_type : globname (* name of containing aggregate *)
 ; f_name : ident
 }.
 #[global] Instance field_eq: EqDecision field.
 Proof. solve_decision. Defined.
+
+(* QUESTION (JH): Should these be sealed? Using what method? *)
+Definition null_memberp_name : ident := "!NULL_MEMBER_PTR".
+Definition null_memberp (cls : globname) : field := Build_field cls null_memberp_name.
